More code lemmas

src/Codes.v
@@ -195,7 +195,7 @@ Proof.
     compute; auto.
   unfold code_sub; fold (@code_sub Var Var').
   red_to ((x1 @ f) * (x2 @ g)).
-Defined.
+Qed.
 Hint Resolve red_sub_left.
 
 Lemma beta_sub_right {Var Var' : Set}
@@ -229,7 +229,7 @@ Lemma red_sub {Var Var' : Set}
   red (code_sub f x) (code_sub g y).
 Proof.
   red_to (code_sub g x).
-Defined.
+Qed.
 Hint Resolve red_sub.
 
 (** Contexts, convergence, and information ordering *)
@@ -289,13 +289,44 @@ Proof.
 Qed.
 Hint Resolve code_le_ap.
 
+Lemma code_le_red_left {Var : Set} (x x' y : Code Var) :
+  red x x' -> x [= y -> x' [= y.
+Proof.
+  unfold code_le; intros Hred Hxy Var' c f Hconv.
+  apply Hxy.
+  red_to (code_div o c * (x @ f)).
+  red_to (code_div o c * (x' @ f)).
+  red_to (code_div * (c * (x' @ f))).
+Qed.
+Hint Resolve code_le_red_left.
+
+Lemma code_le_red_right {Var : Set} (x y y' : Code Var) :
+  red y' y -> x [= y -> x [= y'.
+Proof.
+  unfold code_le; intros Hred Hxy Var' c f Hconv.
+  red_to (code_div o c * (y' @ f)).
+  red_to (code_div o c * (y @ f)).
+  red_to (code_div * (c * (y @ f))).
+  apply Hxy; auto.
+Qed.
+Hint Resolve code_le_red_right.
+
+Lemma code_le_red {Var : Set} (x x' y y' : Code Var) :
+  red x x' -> red y' y -> x [= y -> x' [= y'.
+Proof.
+  intros Hx Hy Hxy.
+    apply code_le_red_right with y; auto.
+  apply code_le_red_left with x; auto.
+Qed.
+Hint Resolve code_le_red.
+
 Lemma code_le_top {Var : Set} (x : Code Var) : x [= TOP.
 Proof.
   unfold code_le; intros Var' c f Hred.
   red_to (code_div o c * TOP).
   red_to (code_div o c * (x @ f)).
   red_to (code_div * (c * (x @ f))).
-Defined.
+Qed.
 Hint Resolve code_le_top.
 
 Lemma code_le_bot {Var : Set} (x : Code Var) : BOT [= x.
@@ -304,7 +335,7 @@ Proof.
   red_to (code_div o c * (x @ f)).
   red_to (code_div o c * BOT).
   red_to (code_div * (c * BOT)).
-Defined.
+Qed.
 Hint Resolve code_le_bot.
 
 Lemma code_le_j_left {Var : Set} (x y : Code Var) : x [= x || y.
@@ -312,16 +343,46 @@ Proof.
   unfold code_le; intros Var' c f Hred.
   red_to (code_div * (c * (x @ f))).
 Qed.
+Hint Resolve code_le_j_left.
 
 Lemma code_le_j_right {Var : Set} (x y : Code Var) : y [= x || y.
 Proof.
   unfold code_le; intros Var' c f Hred.
   red_to (code_div * (c * (y @ f))).
 Qed.
+Hint Resolve code_le_j_right.
 
-Lemma code_le_j {Var : Set} (x y z : Code Var) :
+Lemma code_le_j_ub {Var : Set} (x y z : Code Var) :
   x [= z -> y [= z -> x || y [= z.
 Proof.
-  unfold code_le; intros Hx Hy Var' c f.
+  unfold code_le; unfold conv; intros Hx Hy Var' c f Hconv.
   (* TODO *)
 Admitted.
+Hint Resolve code_le_j_ub.
+
+Lemma code_le_ext {Var : Set} (x x' : Code Var) :
+  (forall y, x * y [= x' * y) -> x [= x'.
+Proof.
+  (* TODO implement via abstraction algorithm *)
+Admitted.
+Hint Resolve code_le_ext.
+
+(** ** Observational equivalence *)
+
+Definition code_eq {Var : Set} (x y : Code Var) := x [= y /\ y [= x.
+Notation "x [=] y" := (code_eq x y)%code : code_scope.
+
+Lemma code_eq_beta {Var : Set} (x y : Code Var) : beta x y -> x [=] y.
+Proof.
+  unfold code_eq; intros Hbeta; split.
+  assert (Hxy : red x y); auto; apply code_le_red_left with y; auto.
+  assert (Hyx : red y x); auto; apply code_le_red_right with y; auto.
+Qed.
+Hint Resolve code_eq_beta.
+
+Lemma code_eq_ext {Var : Set} (x x' : Code Var) :
+  (forall y, x * y [=] x' * y) -> x [=] x'.
+Proof.
+  unfold code_eq; intro H; split; apply code_le_ext; intro y; apply H.
+Qed.
+Hint Resolve code_eq_ext.
